\documentclass[letterpaper,10pt]{article}
\usepackage[margin=64pt]{geometry}
\usepackage{amsthm}
\usepackage{amsmath}
\usepackage{amssymb}
\usepackage{parskip}
\usepackage{graphicx}
\usepackage{enumerate}
\usepackage{hyperref}

\setcounter{secnumdepth}{0}

\newcommand{\doubleu}[1]{\underline{\underline{#1}}}
\newcommand{\ddx}[1]{\frac{d}{dx} \bigg( #1 \bigg)}
\newcommand{\mathematica}[1]{Mathematica: \texttt{#1}}

\begin{document}

	\noindent {\bf Rukmal Weerawarana (1337197)} \newline
	\noindent {\bf CFRM 460} \newline
	\noindent {\bf Homework 1 Solutions} \newline
	\noindent {\bf 1/15/16}
	\newline \hrule


	\section{Question 1}

		\subsection{Part (a)}
			\begin{gather*}
				\lim_{h \rightarrow 0} \frac{4(x+h-3)^2-4(x-3)^2}{h}
				= \lim_{h \rightarrow 0} \frac{4((x+h)^2 - 6(x+h) + 9)-4(x^2-6x+9)}{h} \\
				= \lim_{h \rightarrow 0} \frac{4(x^2+2xh+h^2-6x-6h+9)-4x^2+24x-36}{h} \\
				= \lim_{h \rightarrow 0} \frac{4x^2+8xh+4h^2-24x-24h+36-4x^2+24h-36}{h}
				= \lim_{h \rightarrow 0} \frac{4h^2+8xh-24h}{h} \\
				= \lim_{h \rightarrow 0} (\frac{4h^2}{h} + \frac{8xh}{h} - \frac{24h}{h})
				= 8x - 24 - (\lim_{h \rightarrow 0} 4h) \\
				= \doubleu{8x-24}
			\end{gather*}
			\mathematica{Limit[(4 (x + h - 3)\^{}2 - 4 (x - 3)\^{}2)/h, h -> 0]}

		\subsection{Part (b)}
			\begin{gather*}
				\lim_{x \rightarrow \infty} \frac{1}{\sqrt{4x^2-2x-10}+2x}
				= \lim_{x \rightarrow \infty} \frac{1}{\sqrt{(2x-\frac{1}{2})^2-\frac{41}{4}}+2x}\\
				\text{Thus, it is clear that the denominator of the function will approach infinity as } x \rightarrow \infty \\
				\Rightarrow \lim_{x \rightarrow \infty} \frac{1}{\sqrt{4x^2-2x-10}+2x}
				= \doubleu{0}
			\end{gather*}
			\mathematica{Limit[1/(Sqrt[4 x\^{}2 - 2 x - 10] + 2 x), x -> Infinity]}


	\section{Question 2}

		\subsection{Part (a)}
			\begin{gather*}
				\Rightarrow f'(x) = \ddx{\frac{1}{1-x}}
				= \ddx{(1-x)^{-1}} \\
				\text{Using the chain rule:} \\
				= -(1-x)^{-2} \cdot -1 = \doubleu{\frac{1}{(1-x)^2}}
			\end{gather*}
			\mathematica{D[1/(1 - x), x]}

		\subsection{Part (b)}
			\begin{gather*}
				\Rightarrow f'(x) = \ddx{\sum_{k=1}^{7} k e^{-a_kx^3}}
				= \sum_{k=1}^{7} k \ddx{e^{-a_kx^3}} \\
				\text{Using the chain rule:} \\
				= \sum_{k=1}^{7} k (e^{-a_kx^3} \cdot -3a_kx^2)
				= \doubleu{-3 \sum_{k=1}^{7} ka_kx^2e^{-a_kx^3}}
			\end{gather*}
			\mathematica{D[Sum[k * Exp[-a[k] x\^{}3], \{k, 1, 7\}], x]}

		\subsection{Part (c)}
			\begin{gather*}
				\Rightarrow f'(x) = \ddx{\frac{\log \big(\frac{x}{K}\big) + \Big(r - q + \frac{\sigma^2}{2}\Big)(T-t)}{\sigma\sqrt{T-t}}}
				= \frac{1}{\sigma\sqrt{T-t}} \cdot \ddx{\log \big(\frac{x}{K}\big) + \Big(r - q + \frac{\sigma^2}{2}\Big)(T-t)} \\
				\text{Using the chain rule, and eliminating constants:} \\
				= \frac{1}{\sigma\sqrt{T-t}} \cdot \frac{1}{\frac{x}{K}} \cdot \frac{1}{K}
				= \frac{1}{\sigma\sqrt{T-t}} \cdot \frac{K}{x} \cdot \frac{1}{K}
				= \doubleu{\frac{1}{(\sigma\sqrt{T-t})x}}
			\end{gather*}
			\mathematica{D[(Log[x/K] + (r - q + (\textbackslash[Sigma]\^{}2)/2) (T - t))/(\textbackslash[Sigma] Sqrt[T - t]), x]}

		\subsection{Part (d)}
			\begin{gather*}
				\Rightarrow f'(x) = \ddx{\frac{\log \big(\frac{S}{K}\big) + \Big(r-q+\frac{x^2}{2}\Big) (T-t)}{x\sqrt{T-t}}}
				= \frac{1}{\sqrt{T-t}} \cdot \ddx{\frac{\log \big(\frac{S}{K}\big)}{x} + \frac{\Big(r-q+\frac{x^2}{2}\Big) (T-t)}{x}} \\
				= \frac{1}{\sqrt{T-t}} \Bigg( -\frac{\log \big(\frac{S}{K}\big)}{x^2} + \ddx{\frac{(r-q)(T-t)}{x} + \frac{\frac{x^2}{2}(T-t)}{x}} \Bigg) \\
				= \frac{1}{\sqrt{T-t}} \Bigg( -\frac{\log \big(\frac{S}{K}\big)}{x^2} + \ddx{\frac{(r-q)(T-t)}{x} + \frac{x(T-t)}{2}} \Bigg)
				= \frac{1}{\sqrt{T-t}} \Bigg( -\frac{\log \big(\frac{S}{K}\big)}{x^2} - \frac{(r-q)(T-t)}{x^2} + \frac{(T-t)}{2} \Bigg) \\
				= \doubleu{\frac{\sqrt{T-t}}{2} - \frac{\log \big(\frac{S}{K}\big) + (r-q)(T-t)}{x^2\sqrt{T-t}}}
			\end{gather*}
			\mathematica{D[(Log[S/K] + (r - q + (x\^{}2/2)) (T - t))/(x Sqrt[T - t]), x]}

		\subsection{Part (e)}
			\begin{gather*}
				\Rightarrow f'(x) = \ddx{\frac{\log \big(\frac{S}{K}\big) + (x-q+\frac{\sigma^2}{2})(T-t)}{\sigma\sqrt{T-t}}}
				= \ddx{\frac{\log \big(\frac{S}{K}\big)}{\sigma\sqrt{T-t}} + \frac{(\frac{\sigma^2}{2}-q)(T-t)}{\sigma\sqrt{T-t}} + \frac{x(T-t)}{\sigma\sqrt{T-t}}} \\
				\text{Eliminating constants:} \\
				= \ddx{\frac{x(T-t)}{\sigma\sqrt{T-t}}}
				= \ddx{\frac{x\sqrt{T-t}}{\sigma}}
				= \doubleu{\frac{\sqrt{T-t}}{\sigma}}
			\end{gather*}
			\mathematica{D[(Log[S/K] + (x - q + (\textbackslash[Sigma]\^{}2/2)) (T - t))/(\textbackslash[Sigma] Sqrt[T - t]), x]}


	\section{Question 3}
		\subsection{Part (a)}
			\begin{gather*}
				\lim_{x \rightarrow 0} \frac{\sin (x)}{x} \\
				\text{Thus, as both the numerator and denominator} \rightarrow 0 \text{ as } x \rightarrow 0 \text{, l'H\^opital's rule can be used:} \\
				\Rightarrow \lim_{x \rightarrow 0} \frac{\sin (x)}{x} = \lim_{x \rightarrow 0} \frac{\cos (x)}{1} = \lim_{x \rightarrow 0} \cos (x) = \cos (0) = \doubleu{1}
			\end{gather*}
			\mathematica{Limit[Sin[x]/x, x -> 0]}

		\subsection{Part (b)}
			\begin{gather*}
				\lim_{x \rightarrow \infty} \frac{\log (x^3)}{x}
				= 3 \cdot \lim_{x \rightarrow \infty} \frac{\log (x)}{x} \\
				\text{Thus, as both the numerator and denominator} \rightarrow \infty \text{ as } x \rightarrow \infty \text{, l'H\^opital's rule can be used:} \\
				\Rightarrow 3 \cdot \lim_{x \rightarrow \infty} \frac{\log (x)}{x}
				= 3 \cdot \lim_{x \rightarrow \infty} \frac{\frac{1}{x}}{1}
				= 3 \cdot \lim_{x \rightarrow \infty} \frac{1}{x}
				= 3 \cdot 0
				= \doubleu{0}
			\end{gather*}
			\mathematica{Limit[Log[x\^{}3]/x, x -> Infinity]}

\end{document}
